functordone

theories/SepBase.v
@@ -62,13 +62,48 @@ Definition heap_union_empty_r := fmap_union_empty_r.
 
 Definition heap_union_comm := fmap_union_comm_of_disjoint.
 
-
 (* ---------------------------------------------------------------------- *)
-(** Hprop *)
+(* ** Hprop *)
 
 (** A heap predicate, type [hprop] is a predicate over such heaps. *)
 
 Definition hprop := heap -> Prop.
+
+
+(* ---------------------------------------------------------------------- *)
+(* ** Entailment *)
+
+Definition himpl (H1 H2:hprop) : Prop :=
+  forall (h:heap), H1 h -> H2 h.
+
+Notation "H1 ==> H2" := (himpl H1 H2) (at level 55) : heap_scope.
+
+Local Open Scope heap_scope.
+
+Definition qimpl A (Q1 Q2:A->hprop) : Prop :=
+  forall (v:A), Q1 v ==> Q2 v.
+
+Notation "Q1 ===> Q2" := (qimpl Q1 Q2) (at level 55) : heap_scope.
+
+Lemma himpl_refl : forall H,
+  H ==> H.
+Proof using. introv M. auto. Qed.
+
+Lemma himpl_trans : forall H2 H1 H3,
+  (H1 ==> H2) ->
+  (H2 ==> H3) ->
+  (H1 ==> H3).
+Proof using. introv M1 M2. intros h H1h. eauto. Qed.
+
+Lemma himpl_antisym : forall H1 H2,
+  (H1 ==> H2) ->
+  (H2 ==> H1) ->
+  (H1 = H2).
+Proof using. introv M1 M2. applys pred_ext_1. intros h. iff*. Qed.
+
+
+(* ---------------------------------------------------------------------- *)
+(** Operators *)
 
 (** Affinity is defined in the standard way *)
 
@@ -110,6 +145,8 @@ Notation "H1 '\*' H2" := (hstar H1 H2)
 
 Notation "Q \*+ H" := (fun x => hstar (Q x) H)
   (at level 40) : heap_scope.
+
+Open Scope heap_scope.
 
 
 (* ---------------------------------------------------------------------- *)
@@ -153,7 +190,7 @@ Hint Resolve hempty_intro.
 Lemma hstar_hempty_l : forall H,
   hempty \* H = H.
 Proof using.
-  intros. applys hprop_extens. intros h.
+  intros. applys pred_ext_1. intros h.
   iff (h1&h2&M1&M2&D&U) M.
   { forwards E: hempty_inv M1. subst.
     rewrite~ heap_union_empty_l. }
@@ -170,7 +207,7 @@ Qed.
 Lemma hstar_assoc : forall H1 H2 H3,
   (H1 \* H2) \* H3 = H1 \* (H2 \* H3).
 Proof using.
-  intros H1 H2 H3. applys hprop_extens. intros h. split.
+  intros H1 H2 H3. applys pred_ext_1. intros h. split.
   { intros (h'&h3&(h1&h2&M3&M4&D'&U')&M2&D&U). subst h'.
     exists h1 (h2 \+ h3). splits~. { exists* h2 h3. } }
   { intros (h1&h'&M1&(h2&h3&M3&M4&D'&U')&D&U). subst h'.
@@ -180,7 +217,7 @@ Qed.
 Lemma hstar_hexists : forall A (J:A->hprop) H,
   (hexists J) \* H = hexists (fun x => (J x) \* H).
 Proof using.
-  intros. applys hprop_extens. intros h. iff M.
+  intros. applys pred_ext_1. intros h. iff M.
   { destruct M as (h1&h2&(x&M1)&M2&D&U). exists~ x h1 h2. }
   { destruct M as (x&(h1&h2&M1&M2&D&U)). exists h1 h2. splits~. exists~ x. }
 Qed.
@@ -443,6 +480,214 @@ Ltac simpl_abs := (* LATER: will be removed once [abs] computes *)
   | |- context [ abs 2 ] => change (abs 2) with 2%nat
   | |- context [ abs 3 ] => change (abs 3) with 3%nat
   end.
+
+
+
+(* ********************************************************************** *)
+(** * Definition of Hoare triples *)
+
+Definition hoare (t:trm) (H:hprop) (Q:val->hprop) :=
+  forall h, H h -> exists h' v, eval h t h' v /\ Q v h'.
+
+
+(* ---------------------------------------------------------------------- *)
+(* ** Tactic [himpl_fold] *)
+
+(** [himpl_fold] applies to a goal of the form [H1 h].
+    It searches the context for an assumption of the from [H2 h],
+    then replaces the goal with [H1 ==> H2].
+    It also deletes the assumption [H2 h]. *)
+
+Ltac himpl_fold_core tt :=
+  match goal with N: ?H ?h |- _ ?h =>
+    applys himpl_inv N; clear N end.
+
+Tactic Notation "himpl_fold" := himpl_fold_core tt.
+Tactic Notation "himpl_fold" "~" := himpl_fold; auto_tilde.
+Tactic Notation "himpl_fold" "*" := himpl_fold; auto_star.
+
+
+(* ********************************************************************** *)
+(** * Hoare structural rules *)
+
+Lemma hoare_conseq : forall t H' Q' H Q,
+  hoare t H' Q' ->
+  H ==> H' ->
+  Q' ===> Q ->
+  hoare t H Q.
+Proof using.
+  introv M MH MQ HF. forwards (h'&v&R&K): M h.
+  { himpl_fold~. }
+  exists h' v. splits~. { himpl_fold. auto. }
+Qed.
+
+Lemma hoare_named_heap : forall t H Q,
+  (forall h, H h -> hoare t (= h) Q) ->
+  hoare t H Q.
+Proof using. introv M. intros h Hh. applys* M. Qed.
+
+
+(* ********************************************************************** *)
+(** * Hoare rules for term constructs *)
+
+Lemma hoare_evalctx : forall C t1 H Q Q1,
+  evalctx C ->
+  hoare t1 H Q1 ->
+  (forall v, hoare (C v) (Q1 v) Q) ->
+  hoare (C t1) H Q.
+Proof using.
+  introv HC M1 M2 Hh.
+  forwards* (h1'&v1&R1&K1): (rm M1).
+  forwards* (h2'&v2&R2&K2): (rm M2).
+  exists h2' v2. splits~. { applys~ eval_evalctx R2. }
+Qed.
+
+Lemma hoare_val : forall v H Q,
+  H ==> Q v ->
+  hoare (trm_val v) H Q.
+Proof using.
+  introv M. intros h Hh. exists h v. splits.
+  { applys eval_val. }
+  { himpl_fold~. }
+Qed.
+
+Lemma hoare_fixs : forall f xs t1 H Q,
+  xs <> nil ->
+  H ==> Q (val_fixs f xs t1) ->
+  hoare (trm_fixs f xs t1) H Q.
+Proof using.
+  introv N M. intros h Hh. exists___. splits.
+  { applys~ eval_fixs. }
+  { himpl_fold~. }
+Qed.
+
+Lemma hoare_fun : forall x t1 H Q,
+  H ==> Q (val_fun x t1) ->
+  hoare (trm_fun x t1) H Q.
+Proof using. introv M. applys hoare_fixs; auto_false. Qed.
+
+Lemma hoare_fix : forall f x t1 H Q,
+  H ==> Q (val_fix f x t1) ->
+  hoare (trm_fix f x t1) H Q.
+Proof using. introv M. applys hoare_fixs; auto_false. Qed.
+
+Lemma hoare_constr : forall id vs H Q,
+  H ==> Q (val_constr id vs) ->
+  hoare (trm_constr id (trms_vals vs)) H Q.
+Proof using.
+  introv M. intros h Hh. exists h (val_constr id vs). splits.
+  { applys eval_constr. }
+  { himpl_fold~. }
+Qed.
+
+Lemma hoare_constr_trm : forall id ts t1 vs H Q Q1,
+  hoare t1 H Q1 -> 
+  (forall v, hoare (trm_constr id ((trms_vals vs)++(trm_val v)::ts)) (Q1 v) Q) ->
+  hoare (trm_constr id ((trms_vals vs)++t1::ts)) H Q.
+Proof using.
+  introv M1 M2. intros h Hh.
+  forwards* (h1'&v1&R1&K1): (rm M1).
+  forwards* (h2'&v2&R2&K2): (rm M2).
+  exists h2' v2. splits~. { applys~ eval_constr_trm R2. }
+Qed.
+
+
+Lemma hoare_let : forall z t1 t2 H Q Q1,
+  hoare t1 H Q1 ->
+  (forall v, hoare (subst1 z v t2) (Q1 v) Q) ->
+  hoare (trm_let z t1 t2) H Q.
+Proof using.
+  introv M1 M2 Hh.
+  forwards* (h1'&v1&R1&K1): (rm M1).
+  forwards* (h2'&v2&R2&K2): (rm M2).
+  exists h2' v2. splits~. { applys~ eval_let_trm R2. }
+Qed.
+
+Lemma hoare_seq : forall t1 t2 H Q H1,
+  hoare t1 H (fun r => H1) ->
+  hoare t2 H1 Q ->
+  hoare (trm_seq t1 t2) H Q.
+Proof using. introv M1 M2. applys* hoare_let. Qed.
+
+Lemma hoare_if_case : forall (b:bool) t1 t2 H Q,
+  hoare (if b then t1 else t2) H Q ->
+  hoare (trm_if b t1 t2) H Q.
+Proof using.
+  introv M1. intros h Hh. forwards* (h1'&v1&R1&K1): (rm M1).
+  exists h1' v1. splits~. { applys* eval_if. }
+Qed.
+
+Lemma hoare_if_trm : forall Q1 t0 t1 t2 H Q,
+  hoare t0 H Q1 ->
+  (forall v, hoare (trm_if v t1 t2) (Q1 v) Q) ->
+  hoare (trm_if t0 t1 t2) H Q.
+Proof using.
+  introv M1 M2. applys* hoare_evalctx (fun t0 => trm_if t0 t1 t2).
+  { constructor. }
+Qed.
+
+Lemma hoare_apps_funs : forall xs F vs t1 H Q,
+  F = (val_funs xs t1) ->
+  var_funs (length vs) xs ->
+  hoare (substn xs vs t1) H Q ->
+  hoare (trm_apps F vs) H Q.
+Proof using.
+  introv E N M. intros h Hh. forwards* (h'&v&R&K): (rm M).
+  exists h' v. splits~. { subst. applys* eval_apps_funs. }
+Qed.
+
+Lemma hoare_apps_fixs : forall xs (f:var) F vs t1 H Q,
+  F = (val_fixs f xs t1) ->
+  var_fixs f (length vs) xs ->
+  hoare (substn (f::xs) (F::vs) t1) H Q ->
+  hoare (trm_apps F vs) H Q.
+Proof using.
+  introv E N M. intros h Hh. forwards* (h'&v&R&K): (rm M).
+  exists h' v. splits~. { subst. applys* eval_apps_fixs. }
+Qed.
+
+Lemma hoare_while_raw : forall t1 t2 H Q,
+  hoare (trm_if t1 (trm_seq t2 (trm_while t1 t2)) val_unit) H Q ->
+  hoare (trm_while t1 t2) H Q.
+Proof using.
+  introv M Hh. forwards* (h1'&v1&R1&K1): (rm M).
+  exists h1' v1. splits~. { applys* eval_while. }
+Qed.
+
+Lemma hoare_for_raw : forall (x:var) (n1 n2:int) t3 H Q,
+  hoare (
+    If (n1 <= n2)
+      then (trm_seq (subst1 x n1 t3) (trm_for x (n1+1) n2 t3))
+      else val_unit) H Q ->
+  hoare (trm_for x n1 n2 t3) H Q.
+Proof using.
+  introv M Hh. forwards* (h1'&v1&R1&K1): (rm M).
+  exists h1' v1. splits~. { applys* eval_for. }
+Qed.
+
+Lemma hoare_match : forall v p t1 pts H Q,
+  (forall (G:ctx), Ctx.dom G = patvars p -> v = patsubst G p -> hoare (isubst G t1) H Q) ->
+  ((forall (G:ctx), Ctx.dom G = patvars p -> v <> patsubst G p) -> hoare (trm_match v pts) H Q) ->
+  hoare (trm_match v ((p,t1)::pts)) H Q.
+Proof using.
+  introv M1 M2 Hh. tests C: (exists (G:ctx), Ctx.dom G = patvars p /\ v = patsubst G p).
+  { destruct C as (G&DG&Ev). forwards* (h1'&v1&R1&K1): (rm M1).
+    exists h1' v1. splits~. { applys~ eval_match_yes R1. } }
+  { forwards* (h1'&v1&R1&K1): (rm M2).
+    exists h1' v1. splits~. { applys~ eval_match_no R1.
+      intros G HG. specializes C G. rew_logic in C. destruct* C. } }
+Qed.
+
+Lemma hoare_case_trm : forall t1 pts H Q Q1,
+  hoare t1 H Q1 -> 
+  (forall v, hoare (trm_match v pts) (Q1 v) Q) ->
+  hoare (trm_match t1 pts) H Q.
+Proof using.
+  introv M1 M2. intros h Hh.
+  forwards* (h1'&v1&R1&K1): (rm M1).
+  forwards* (h2'&v2&R2&K2): (rm M2).
+  exists h2' v2. splits~. { applys~ eval_match_trm R2. }
+Qed.
 
 
 (* ********************************************************************** *)
