extra/Entail.v
@@ -1,0 +1,125 @@
+(**
+
+This file formalizes entailement, written [H ==> H'], and its generalization
+to postconditions, written [Q ===> Q'].
+
+Author: Arthur Charguéraud.
+License: MIT.
+
+*)
+
+Set Implicit Arguments.
+From Sep Require Export Semantics.
+Open Scope fmap_scope.
+
+
+(* ********************************************************************** *)
+(** * Entailment *)
+
+(** The definition of entailment is polymorphic in the type of heaps,
+    which could be state, but also more elaborated structures in
+    extensions of Separation Logic (e.g. with time credits). *)
+
+
+(* ---------------------------------------------------------------------- *)
+(* ** Predicate extensionality, specialized to heap predicates *)
+
+(** Predicate extensionality follows from functional extensional
+    and propositional extensionality, which we take as axiom
+    (in TLC's LibAxioms file). *)
+
+Lemma hprop_extens : forall A (H1 H2:A->Prop),
+  (forall h, H1 h <-> H2 h) ->
+  (H1 = H2).
+Proof using.
+  introv M. applys fun_ext_1. intros h. applys* prop_ext.
+Qed.
+
+(* ---------------------------------------------------------------------- *)
+(* ** Definition of entailment *)
+
+(** [H1 ==> H2] is defined as [forall h, H1 h -> H2 h]. *)
+
+Definition himpl A (H1 H2:A->Prop) :=
+  forall x, H1 x -> H2 x.
+
+Notation "H1 ==> H2" := (himpl H1 H2)
+  (at level 55) : heap_scope.
+
+(** [Q1 ===> Q2] is defined as [forall x h, Q1 x h -> Q2 x h].
+    It is thus equivalent to [forall x, Q1 x ==> Q2 x].
+    Thus, invoking [intro] on a [===>] goal leaves a [==>] goal. *)
+
+Definition qimpl A B (Q1 Q2:A->B->Prop) :=
+  forall r, himpl (Q1 r) (Q2 r).
+
+Notation "Q1 ===> Q2" := (qimpl Q1 Q2)
+  (at level 55) : heap_scope.
+
+Open Scope heap_scope.
+
+
+(* ---------------------------------------------------------------------- *)
+(* ** Properties of entailment *)
+
+Section HimplProp.
+Variable A : Type.
+Implicit Types H : A -> Prop.
+
+Hint Unfold himpl.
+
+(** Entailment is reflexive, symmetric, transitive *)
+
+Lemma himpl_refl : forall H,
+  H ==> H.
+Proof using. intros h. auto. Qed.
+
+Lemma himpl_trans : forall H2 H1 H3,
+  (H1 ==> H2) ->
+  (H2 ==> H3) ->
+  (H1 ==> H3).
+Proof using. introv M1 M2. intros h H1h. eauto. Qed.
+
+Lemma himpl_antisym : forall H1 H2,
+  (H1 ==> H2) ->
+  (H2 ==> H1) ->
+  (H1 = H2).
+Proof using. introv M1 M2. applys pred_ext_1. intros h. iff*. Qed.
+
+(** Paragraphe of the definition, used by tactics *)
+
+Lemma himpl_inv : forall H1 H2 (h:A),
+  (H1 ==> H2) ->
+  (H1 h) ->
+  (H2 h).
+Proof using. auto. Qed.
+
+(** Reformulation of reflexivity, used by tactics *)
+
+Lemma himpl_of_eq : forall H1 H2,
+  H1 = H2 ->
+  H1 ==> H2.
+Proof. intros. subst. applys~ himpl_refl. Qed.
+
+Lemma himpl_of_eq_sym : forall H1 H2,
+  H1 = H2 ->
+  H2 ==> H1.
+Proof. intros. subst. applys~ himpl_refl. Qed.
+
+End HimplProp.
+
+Arguments himpl_of_eq [A] [H1] [H2].
+Arguments himpl_of_eq_sym [A] [H1] [H2].
+Arguments himpl_antisym [A] [H1] [H2].
+
+Hint Resolve himpl_refl.
+
+(** Reflexivity for postconditions *)
+
+Lemma qimpl_refl : forall A B (Q:A->B->Prop),
+  Q ===> Q.
+Proof using. intros. hnfs*. Qed.
+
+Hint Resolve qimpl_refl.
+
+
